proofs/Gcd.lean
@@ -1,19 +1,51 @@
+-- This module serves as the root of the `Gcd` library.
+-- Import modules here that should be built as part of the library.
 import Gcd.Funs
+
 open Aeneas.Std Result Error
 namespace gcd
 
-theorem euclid_loop0_u8_spec (a b : U8)
-  : ∃ y, euclid_u8_loop0 a b = ok y
-  := by
-  unfold euclid_u8_loop0
-  split
-  case isTrue h =>
-    have : b ≠ 0#u8 := by grind
-    progress as ⟨ c ⟩
-    progress
-  case isFalse h =>
-    simp
-termination_by b
-decreasing_by
-  unfold sizeOf UScalar._sizeOf_inst UScalar._sizeOf_1
-  aesop (add safe Nat.mod_lt) (add safe Nat.pos_of_ne_zero)
+attribute [scalar_tac_simps] bne_iff_ne
+
+@[progress]
+theorem euclid_loop_u8_spec (a b : U8) :
+    ∃ y, euclid_u8_loop a b = ok y := by
+  unfold euclid_u8_loop
+  progress*
+termination_by b.val
+decreasing_by scalar_tac
+
+theorem euclid_u8_spec (a b : U8) :
+    ∃ y, euclid_u8 a b = ok y := by
+  unfold euclid_u8
+  progress*
+
+axiom trailing_zeros : U8 → U32
+
+@[progress]
+theorem trailing_zeros_spec (v : U8) (hv : v ≠ 0#u8):
+  ∃ y, core.num.U8.trailing_zeros v = .ok y ∧ y < 8#u32 ∧ y = trailing_zeros v := sorry
+
+@[progress]
+theorem shift_right_spec (u : U8) (v : U32) (hu : u ≠ 0#u8) (hv : v ≤ trailing_zeros u):
+  ∃ y, u >>> v = .ok y ∧ y ≠ 0#u8 ∧ y ≤ u := sorry
+
+@[progress]
+theorem bor_spec (u v : U8) (hu : u ≠ 0#u8) (hv : v ≠ 0#u8) :
+  ∃ y, (↑(u ||| v) : Result U8) = .ok y ∧
+    trailing_zeros y ≤ trailing_zeros u ∧
+    trailing_zeros y ≤ trailing_zeros v ∧
+    y ≠ 0#u8 := sorry
+
+@[progress]
+theorem binary_u8_loop_spec (a b : U8) (ha : a ≠ 0#u8) (hb : b ≠ 0#u8):
+    ∃ y, binary_u8_loop a b = ok y ∧ y ≠ 0#u8 := by
+  unfold binary_u8_loop
+  progress*
+termination_by a.val + b.val
+decreasing_by all_goals scalar_tac
+
+theorem binary_u8_spec (a b : U8) :
+    ∃ y, binary_u8 a b = ok y := by
+  unfold binary_u8
+  progress*
