README_AENEAS.md
@@ -1,7 +1,0 @@
-This is how to extract Lean via Aeneas:
-```
-../aeneas/charon/bin/charon cargo --preset=aeneas
-../aeneas/bin/aeneas -backend lean -dest proofs/GcdVerif -split-files ./gcd.llbc
-```
-
-TH `split-files` option allows us to define our own library functions, in particular the function `trailing_zeros` that is missing.
